LOG2 is now defined using James' logrootTheory.  Other simplifications have also been made, following some recent additions to arithmeticTheory.

src/n-bit/bitScript.sml
@@ -5,8 +5,12 @@
 (* DATE          : 2000-2005                                                 *)
 (* ========================================================================= *)
 
+(* interactive use:
+  load "logrootTheory";
+*)
+
 open HolKernel Parse boolLib bossLib;
-open Q simpLib numLib arithmeticTheory prim_recTheory;
+open Q simpLib numLib arithmeticTheory logrootTheory prim_recTheory;
 
 val _ = new_theory "bit";
 
@@ -77,7 +81,18 @@ val SIGN_EXTEND_def =
          let m = n MOD 2 ** l in
          if BIT (l - 1) n then 2 ** h - 2 ** l + m else m`;
 
+val LOG2_def = Def "LOG2_def" `LOG2 = LOG 2`;
+
+val LOG2_UNIQUE = save_thm("LOG2_UNIQUE",
+  (REWRITE_RULE [GSYM LOG2_def] o INST [`a` |-> `2`]) LOG_UNIQUE);
+
 (* ------------------------------------------------------------------------- *)
+
+infix \\ << >>
+
+val op \\ = op THEN;
+val op << = op THENL;
+val op >> = op THEN1;
 
 val LEFT_REWRITE_TAC =
   GEN_REWRITE_TAC (RATOR_CONV o DEPTH_CONV) empty_rewrites;
@@ -113,30 +128,15 @@ val th = (SPEC_ALL o REWRITE_RULE [ZERO_LT_TWOEXP] o SPEC `2 ** n`) DIVISION;
 val MOD_2EXP_LT = save_thm("MOD_2EXP_LT", (GEN_ALL o CONJUNCT2) th);
 
 (* |- !n k. k = k DIV 2 ** n * 2 ** n + k MOD 2 ** n *)
-val TWOEXP_DIVISION = save_thm("TWOEXP_DIVISION",
-  (GEN_ALL o CONJUNCT1) th);
+val TWOEXP_DIVISION = save_thm("TWOEXP_DIVISION", (GEN_ALL o CONJUNCT1) th);
 
-val MULT_INCREASES2 = ONCE_REWRITE_RULE [MULT_COMM]
-  (REWRITE_RULE [GSYM LESS_EQ] MULT_INCREASES);
-
-val ONE_LT_TWOEXP_SUCN = prove(
-  `!n. 1 < 2 ** n * 2`,
-  Induct_on `n` THEN RW_TAC arith_ss [EXP,MULT_INCREASES2]);
-
-val TWOEXP_MONO = store_thm("TWOEXP_MONO",
-  `!a b. a < b ==> 2 ** a < 2 ** b`,
-  REPEAT STRIP_TAC
-    THEN IMP_RES_TAC LESS_ADD_1
-    THEN ASM_SIMP_TAC arith_ss [EXP_ADD,MULT_INCREASES2,
-           ONE_LT_TWOEXP_SUCN,ZERO_LT_TWOEXP]);
-
-val TWOEXP_MONO2 = store_thm("TWOEXP_MONO2",
-  `!a b. a <= b ==> 2 ** a <= 2 ** b`,
-  REPEAT STRIP_TAC
-    THEN Cases_on `b = a`
-    THEN FULL_SIMP_TAC arith_ss [GSYM NOT_LESS]
-    THEN IMP_RES_TAC LESS_CASES_IMP
-    THEN RW_TAC bool_ss [TWOEXP_MONO,NOT_LESS,LESS_IMP_LESS_OR_EQ]);
+local
+  val sp2 = GEN `a` o GEN `b` o fst o EQ_IMP_RULE o
+            SPEC_ALL o SIMP_RULE std_ss [] o SPEC `2`
+in
+  val TWOEXP_MONO  = save_thm("TWOEXP_MONO",  sp2 LT_EXP_ISO)
+  val TWOEXP_MONO2 = save_thm("TWOEXP_MONO2", sp2 LE_EXP_ISO)
+end;
 
 val EXP_SUB_LESS_EQ = store_thm("EXP_SUB_LESS_EQ",
   `!a b. 2 ** (a - b) <= 2 ** a`,
@@ -153,8 +153,8 @@ val BITSLT_THM = store_thm("BITSLT_THM",
 
 val DIV_MULT_LEM = prove(
   `!m n. 0 < n ==> m DIV n * n <= m`,
-  RW_TAC arith_ss [LESS_EQ_EXISTS] THEN EXISTS_TAC `m MOD n`
-    THEN RW_TAC arith_ss [GSYM DIVISION]);
+  RW_TAC arith_ss [LESS_EQ_EXISTS] \\ EXISTS_TAC `m MOD n`
+    \\ RW_TAC arith_ss [GSYM DIVISION]);
 
 (* |- !x n. n DIV 2 ** x * 2 ** x <= n *)
 val DIV_MULT_LESS_EQ = GEN_ALL (SIMP_RULE bool_ss [ZERO_LT_TWOEXP]
@@ -174,55 +174,54 @@ val MOD_EXP_ADD = prove(
   `!a b p. a MOD 2 ** (b + p) =
       a MOD 2 ** b + (a DIV 2 ** b) MOD 2 ** p * 2 ** b`,
   REPEAT STRIP_TAC
-    THEN SIMP_TAC bool_ss [MOD_2EXP_LEM,RIGHT_SUB_DISTRIB,DIV_DIV_DIV_MULT,
-           ZERO_LT_TWOEXP,GSYM MULT_ASSOC,GSYM EXP_ADD]
-    THEN ASSUME_TAC ( (GSYM o SPECL [`a DIV 2 ** (b + p) * 2 ** (p + b)`,
-           `a DIV 2 ** b * 2 ** b`]) LESS_EQ_ADD_SUB)
-    THEN ASM_SIMP_TAC arith_ss [DIV_MULT_LEM2,DIV_MULT_LEM,
-           ZERO_LT_TWOEXP,SUB_ADD]);
+    \\ SIMP_TAC bool_ss [MOD_2EXP_LEM,RIGHT_SUB_DISTRIB,DIV_DIV_DIV_MULT,
+         ZERO_LT_TWOEXP,GSYM MULT_ASSOC,GSYM EXP_ADD]
+    \\ ASSUME_TAC ( (GSYM o SPECL [`a DIV 2 ** (b + p) * 2 ** (p + b)`,
+         `a DIV 2 ** b * 2 ** b`]) LESS_EQ_ADD_SUB)
+    \\ ASM_SIMP_TAC arith_ss [DIV_MULT_LEM2,DIV_MULT_LEM,
+         ZERO_LT_TWOEXP,SUB_ADD]);
 
-val DIV_MOD_MOD_DIV = prove(
-  `!a b p. (a DIV 2 ** b) MOD 2 ** p = a MOD 2 ** (b + p) DIV 2 ** b`,
-  RW_TAC arith_ss [MOD_EXP_ADD,ADD_DIV_ADD_DIV,ZERO_LT_TWOEXP,
-    LESS_DIV_EQ_ZERO,DIVISION]);
+val DIV_MOD_MOD_DIV2 = (SIMP_RULE std_ss [ZERO_LT_TWOEXP,GSYM EXP_ADD] o
+  SPECL [`a`,`2 ** b`,`2 ** p`]) DIV_MOD_MOD_DIV;
 
-val DIV_MOD_MOD_DIV2 = prove(
+val DIV_MOD_MOD_DIV3 = prove(
   `!a b c. (a DIV 2 ** b) MOD 2 ** (c - b) = (a MOD 2 ** c) DIV 2 ** b`,
-  REPEAT STRIP_TAC THEN Cases_on `c <= b`
-    THENL [
-      POP_ASSUM (fn th => REWRITE_TAC [REWRITE_RULE [GSYM SUB_EQ_0] th,EXP,MOD_1]
-                            THEN ASSUME_TAC (MATCH_MP TWOEXP_MONO2 th))
-        THEN ASSUME_TAC (SPECL [`c`,`a`] MOD_2EXP_LT)
-        THEN IMP_RES_TAC LESS_LESS_EQ_TRANS
-        THEN ASM_SIMP_TAC bool_ss [LESS_DIV_EQ_ZERO],
+  REPEAT STRIP_TAC \\ Cases_on `c <= b`
+    << [
+      POP_ASSUM (fn th =>
+             REWRITE_TAC [REWRITE_RULE [GSYM SUB_EQ_0] th,EXP,MOD_1]
+               \\ ASSUME_TAC (MATCH_MP TWOEXP_MONO2 th))
+        \\ ASSUME_TAC (SPECL [`c`,`a`] MOD_2EXP_LT)
+        \\ IMP_RES_TAC LESS_LESS_EQ_TRANS
+        \\ ASM_SIMP_TAC bool_ss [LESS_DIV_EQ_ZERO],
       RULE_ASSUM_TAC (REWRITE_RULE [NOT_LESS_EQUAL])
-        THEN IMP_RES_TAC LESS_ADD
-        THEN POP_ASSUM (fn th => SIMP_TAC arith_ss [SYM th,DIV_MOD_MOD_DIV])]);
+        \\ IMP_RES_TAC LESS_ADD
+        \\ POP_ASSUM (fn th => SIMP_TAC arith_ss [SYM th,DIV_MOD_MOD_DIV2])]);
 
 val BITS_THM2 = store_thm("BITS_THM2",
   `!h l n. BITS h l n = (n MOD 2 ** SUC h) DIV 2 ** l`,
-  RW_TAC bool_ss [BITS_THM,DIV_MOD_MOD_DIV2]);
+  RW_TAC bool_ss [BITS_THM,DIV_MOD_MOD_DIV3]);
 
 val BITS_COMP_LEM = prove(
   `!h1 l1 h2 l2 n. h2 + l1 <= h1 ==>
     (((n DIV 2 ** l1) MOD 2 ** (h1 - l1) DIV 2 ** l2) MOD 2 ** (h2 - l2) =
       (n DIV 2 ** (l2 + l1)) MOD 2 ** ((h2 + l1) - (l2 + l1)))`,
   REPEAT STRIP_TAC
-    THEN REWRITE_TAC [SPECL [`(n DIV 2 ** l1) MOD 2 ** (h1 - l1)`,
-           `l2`,`h2`] DIV_MOD_MOD_DIV2]
-    THEN IMP_RES_TAC LESS_EQUAL_ADD
-    THEN POP_ASSUM (fn th => SIMP_TAC arith_ss
-           [EXP_ADD,MOD_MULT_MOD,ZERO_LT_TWOEXP,th])
-    THEN REWRITE_TAC [DIV_MOD_MOD_DIV]
-    THEN SIMP_TAC arith_ss [DIV_DIV_DIV_MULT,ZERO_LT_TWOEXP,GSYM EXP_ADD]
-    THEN REWRITE_TAC [SIMP_RULE arith_ss []
-           (SPECL [`n`,`l1 + l2`,`h2 + l1`] DIV_MOD_MOD_DIV2)]);
+    \\ REWRITE_TAC [SPECL [`(n DIV 2 ** l1) MOD 2 ** (h1 - l1)`,
+         `l2`,`h2`] DIV_MOD_MOD_DIV3]
+    \\ IMP_RES_TAC LESS_EQUAL_ADD
+    \\ POP_ASSUM (fn th => SIMP_TAC arith_ss
+         [EXP_ADD,MOD_MULT_MOD,ZERO_LT_TWOEXP,th])
+    \\ REWRITE_TAC [DIV_MOD_MOD_DIV2]
+    \\ SIMP_TAC arith_ss [DIV_DIV_DIV_MULT,ZERO_LT_TWOEXP,GSYM EXP_ADD]
+    \\ REWRITE_TAC [SIMP_RULE arith_ss []
+         (SPECL [`n`,`l1 + l2`,`h2 + l1`] DIV_MOD_MOD_DIV3)]);
 
 val BITS_COMP_THM = store_thm("BITS_COMP_THM",
   `!h1 l1 h2 l2 n. h2 + l1 <= h1 ==>
      (BITS h2 l2 (BITS h1 l1 n) = BITS (h2+l1) (l2+l1) n)`,
-  REPEAT STRIP_TAC THEN IMP_RES_TAC LESS_EQ_MONO
-    THEN FULL_SIMP_TAC bool_ss [BITS_THM,GSYM ADD_CLAUSES,BITS_COMP_LEM]);
+  REPEAT STRIP_TAC \\ IMP_RES_TAC LESS_EQ_MONO
+    \\ FULL_SIMP_TAC bool_ss [BITS_THM,GSYM ADD_CLAUSES,BITS_COMP_LEM]);
 
 val BITS_DIV_THM = store_thm("BITS_DIV_THM",
   `!h l x n. (BITS h l x) DIV 2 ** n = BITS h (l + n) x`,
@@ -236,12 +235,12 @@ val BITS_LT_HIGH = store_thm("BITS_LT_HIGH",
 
 val BITS_ZERO = store_thm("BITS_ZERO",
   `!h l n. h < l ==> (BITS h l n = 0)`,
-  REPEAT STRIP_TAC THEN IMP_RES_TAC LESS_ADD_1
-    THEN POP_ASSUM (fn th => REWRITE_TAC [th])
-    THEN ASSUME_TAC ((REWRITE_RULE [EXP,SUB,SUB_EQUAL_0] o
-           ONCE_REWRITE_RULE [SUB_PLUS] o REWRITE_RULE [ADD1] o
-           SPECL [`h`,`h + 1 + p`,`n`]) BITSLT_THM)
-    THEN FULL_SIMP_TAC arith_ss []);
+  REPEAT STRIP_TAC \\ IMP_RES_TAC LESS_ADD_1
+    \\ POP_ASSUM (fn th => REWRITE_TAC [th])
+    \\ ASSUME_TAC ((REWRITE_RULE [EXP,SUB,SUB_EQUAL_0] o
+         ONCE_REWRITE_RULE [SUB_PLUS] o REWRITE_RULE [ADD1] o
+         SPECL [`h`,`h + 1 + p`,`n`]) BITSLT_THM)
+    \\ FULL_SIMP_TAC arith_ss []);
 
 val BITS_ZERO2 = store_thm("BITS_ZERO2",
   `!h l. BITS h l 0 = 0`,
@@ -270,13 +269,13 @@ val BIT_B = store_thm("BIT_B",
 val BIT_B_NEQ = store_thm("BIT_B_NEQ",
   `!a b. ~(a = b) ==> ~BIT a (2 ** b)`,
   NTAC 3 STRIP_TAC
-    THEN REWRITE_TAC [BIT_def,BITS_THM,SUC_SUB,EXP_1]
-    THEN IMP_RES_TAC (DECIDE ``!(a:num) b. ~(a = b) ==> (a < b) \/ (b < a)``)
-    THENL [
+    \\ REWRITE_TAC [BIT_def,BITS_THM,SUC_SUB,EXP_1]
+    \\ IMP_RES_TAC (DECIDE ``!(a:num) b. ~(a = b) ==> (a < b) \/ (b < a)``)
+    << [
       IMP_RES_TAC LESS_ADD_1
-        THEN ASM_SIMP_TAC arith_ss [ONCE_REWRITE_RULE [MULT_COMM] MULT_DIV,
-               EXP_ADD,MOD_EQ_0,ZERO_LT_TWOEXP],
-      IMP_RES_TAC TWOEXP_MONO THEN ASM_SIMP_TAC arith_ss [LESS_DIV_EQ_ZERO]]);
+        \\ ASM_SIMP_TAC arith_ss [ONCE_REWRITE_RULE [MULT_COMM] MULT_DIV,
+             EXP_ADD,MOD_EQ_0,ZERO_LT_TWOEXP],
+      IMP_RES_TAC TWOEXP_MONO \\ ASM_SIMP_TAC arith_ss [LESS_DIV_EQ_ZERO]]);
 
 (* ------------------------------------------------------------------------- *)
 
@@ -284,24 +283,24 @@ val BITS_COMP_THM2 = store_thm("BITS_COMP_THM2",
   `!h1 l1 h2 l2 n. BITS h2 l2 (BITS h1 l1 n) =
       BITS (MIN h1 (h2 + l1)) (l2 + l1) n`,
   RW_TAC bool_ss [MIN_DEF,REWRITE_RULE [GSYM NOT_LESS] BITS_COMP_THM]
-    THEN Cases_on `h2 = 0` THEN1 FULL_SIMP_TAC arith_ss [BITS_ZERO,BITS_ZERO2]
-    THEN RULE_ASSUM_TAC (REWRITE_RULE [NOT_ZERO_LT_ZERO])
-    THEN Cases_on `h1 < l1` THEN1 FULL_SIMP_TAC arith_ss [BITS_ZERO,BITS_ZERO2]
-    THEN RULE_ASSUM_TAC (ONCE_REWRITE_RULE [ADD_COMM])
-    THEN IMP_RES_TAC SUB_RIGHT_LESS
-    THEN POP_ASSUM (fn th => ASSUME_TAC
+    \\ Cases_on `h2 = 0` >> FULL_SIMP_TAC arith_ss [BITS_ZERO,BITS_ZERO2]
+    \\ RULE_ASSUM_TAC (REWRITE_RULE [NOT_ZERO_LT_ZERO])
+    \\ Cases_on `h1 < l1` >> FULL_SIMP_TAC arith_ss [BITS_ZERO,BITS_ZERO2]
+    \\ RULE_ASSUM_TAC (ONCE_REWRITE_RULE [ADD_COMM])
+    \\ IMP_RES_TAC SUB_RIGHT_LESS
+    \\ POP_ASSUM (fn th => ASSUME_TAC
            (MATCH_MP TWOEXP_MONO (ONCE_REWRITE_RULE [GSYM LESS_MONO_EQ] th)))
-    THEN ASSUME_TAC (SPECL [`h1`,`l1`,`n`] BITSLT_THM)
-    THEN Cases_on `h1 = l1`
-    THENL [
+    \\ ASSUME_TAC (SPECL [`h1`,`l1`,`n`] BITSLT_THM)
+    \\ Cases_on `h1 = l1`
+    << [
       FULL_SIMP_TAC arith_ss [SYM ONE,SUC_SUB]
-        THEN `BITS h1 l1 n < 2 ** SUC h2` by IMP_RES_TAC LESS_TRANS
-        THEN ASM_SIMP_TAC arith_ss [BITS_LT_HIGH,BITS_DIV_THM],
+        \\ `BITS h1 l1 n < 2 ** SUC h2` by IMP_RES_TAC LESS_TRANS
+        \\ ASM_SIMP_TAC arith_ss [BITS_LT_HIGH,BITS_DIV_THM],
       `~(h1 <= l1)` by DECIDE_TAC
-        THEN POP_ASSUM (fn th => RULE_ASSUM_TAC
+        \\ POP_ASSUM (fn th => RULE_ASSUM_TAC
                (SIMP_RULE bool_ss [th,SUB_LEFT_SUC]))
-        THEN `BITS h1 l1 n < 2 ** SUC h2` by IMP_RES_TAC LESS_TRANS
-        THEN ASM_SIMP_TAC arith_ss [BITS_LT_HIGH,BITS_DIV_THM]]);
+        \\ `BITS h1 l1 n < 2 ** SUC h2` by IMP_RES_TAC LESS_TRANS
+        \\ ASM_SIMP_TAC arith_ss [BITS_LT_HIGH,BITS_DIV_THM]]);
 
 (* ------------------------------------------------------------------------- *)
 
@@ -322,8 +321,8 @@ RW_TAC arith_ss [BIT_def, BITS_COMP_THM]);
 val BIT_SHIFT_THM = Q.store_thm (
 "BIT_SHIFT_THM",
 `!n a s. BIT (n + s) (a * 2 ** s) = BIT n a`,
-RW_TAC std_ss [BIT_def, BITS_def,MOD_2EXP_def, DIV_2EXP_def] THEN
-RW_TAC arith_ss [SUC_SUB, EXP_ADD] THEN
+RW_TAC std_ss [BIT_def, BITS_def,MOD_2EXP_def, DIV_2EXP_def] \\
+RW_TAC arith_ss [SUC_SUB, EXP_ADD] \\
 metisLib.METIS_TAC [GSYM DIV_DIV_DIV_MULT, ZERO_LT_TWOEXP,
                     MULT_DIV, MULT_SYM]);
 
@@ -335,22 +334,16 @@ RW_TAC arith_ss [GSYM (Q.SPECL [`n-s`, `a`, `s`] BIT_SHIFT_THM)]);
 val BIT_SHIFT_THM3 = Q.store_thm (
 "BIT_SHIFT_THM3",
 `!n a s. (n < s) ==> ~BIT n (a * 2 ** s)`,
-RW_TAC std_ss [BIT_def, BITS_def,MOD_2EXP_def, DIV_2EXP_def] THEN
-RW_TAC arith_ss [SUC_SUB, NOT_MOD2_LEM2, GSYM EVEN_MOD2] THEN
-RW_TAC arith_ss [DIV_P, ZERO_LT_TWOEXP] THEN
-Q.EXISTS_TAC `a * 2 ** (s - n)` THEN Q.EXISTS_TAC `0` THEN
+RW_TAC std_ss [BIT_def, BITS_def,MOD_2EXP_def, DIV_2EXP_def] \\
+RW_TAC arith_ss [SUC_SUB, NOT_MOD2_LEM2, GSYM EVEN_MOD2] \\
+RW_TAC arith_ss [DIV_P, ZERO_LT_TWOEXP] \\
+Q.EXISTS_TAC `a * 2 ** (s - n)` \\ Q.EXISTS_TAC `0` \\
 RW_TAC arith_ss [ZERO_LT_TWOEXP,GSYM MULT_ASSOC, GSYM EXP_ADD, EVEN_MULT,
                  EVEN_EXP])
 
 val BIT_OF_BITS_THM2 = store_thm("BIT_OF_BITS_THM2",
   `!h l x n.  h < l + x ==> ~BIT x (BITS h l n)`,
   RW_TAC arith_ss [MIN_DEF,BIT_def,BITS_COMP_THM2,BITS_ZERO]);
-
-(* ------------------------------------------------------------------------- *)
-
-val LSB_ODD = store_thm("LSB_ODD", `LSB = ODD`,
-  ONCE_REWRITE_TAC [FUN_EQ_THM]
-    THEN SIMP_TAC arith_ss [ODD_MOD2_LEM,LSB_def,BIT_def,BITS_THM2,EXP,DIV_1]);
 
 (* ------------------------------------------------------------------------- *)
 
@@ -365,11 +358,11 @@ val DIV_MULT_THM2 = save_thm("DIV_MULT_THM2",
 val LESS_EQ_EXP_MULT = store_thm("LESS_EQ_EXP_MULT",
   `!a b. a <= b ==> ?p. 2 ** b = p * 2 ** a`,
   REPEAT STRIP_TAC
-    THEN IMP_RES_TAC LESS_EQUAL_ADD
-    THEN RULE_ASSUM_TAC (ONCE_REWRITE_RULE [SIMP_RULE arith_ss []
-           (SPEC `2` (GSYM EXP_INJECTIVE))])
-    THEN EXISTS_TAC `2 ** p`
-    THEN FULL_SIMP_TAC arith_ss [EXP_ADD,MULT_COMM]);
+    \\ IMP_RES_TAC LESS_EQUAL_ADD
+    \\ RULE_ASSUM_TAC (ONCE_REWRITE_RULE [SIMP_RULE arith_ss []
+         (SPEC `2` (GSYM EXP_INJECTIVE))])
+    \\ EXISTS_TAC `2 ** p`
+    \\ FULL_SIMP_TAC arith_ss [EXP_ADD,MULT_COMM]);
 
 val LESS_EXP_MULT = SIMP_PROVE bool_ss [LESS_IMP_LESS_OR_EQ,LESS_EQ_EXP_MULT]
   ``!a b. a < b ==> ?p. 2 ** b = p * 2 ** a``;
@@ -380,55 +373,55 @@ val SLICE_LEM1 = prove(
   `!a x y. a DIV 2 ** (x + y) * 2 ** (x + y) =
        a DIV 2 ** x * 2 ** x - (a DIV 2 ** x) MOD 2 ** y * 2 ** x`,
   REPEAT STRIP_TAC
-    THEN REWRITE_TAC [EXP_ADD]
-    THEN SUBST_OCCS_TAC [([2],SPECL [`2 ** x`,`2 ** y`] MULT_COMM)]
-    THEN SIMP_TAC bool_ss [ZERO_LT_TWOEXP,GSYM DIV_DIV_DIV_MULT,MULT_ASSOC,
-           SPECL [`y`,`a DIV 2 ** x`] DIV_MULT_THM,RIGHT_SUB_DISTRIB]);
+    \\ REWRITE_TAC [EXP_ADD]
+    \\ SUBST_OCCS_TAC [([2],SPECL [`2 ** x`,`2 ** y`] MULT_COMM)]
+    \\ SIMP_TAC bool_ss [ZERO_LT_TWOEXP,GSYM DIV_DIV_DIV_MULT,MULT_ASSOC,
+         SPECL [`y`,`a DIV 2 ** x`] DIV_MULT_THM,RIGHT_SUB_DISTRIB]);
 
 val SLICE_LEM2 = prove(
   `!a x y. n MOD 2 ** (x + y) =
            n MOD 2 ** x + (n DIV 2 ** x) MOD 2 ** y * 2 ** x`,
   REPEAT STRIP_TAC
-    THEN SIMP_TAC bool_ss [DIV_MULT_LESS_EQ,MOD_2EXP_LEM,SLICE_LEM1,
-           RIGHT_SUB_DISTRIB,SUB_SUB,SUB_LESS_EQ]
-    THEN Cases_on `n = n DIV 2 ** x * 2 ** x`
-    THEN1 POP_ASSUM (fn th => SIMP_TAC arith_ss [SYM th])
-    THEN ASSUME_TAC (REWRITE_RULE [GSYM NOT_LESS] DIV_MULT_LESS_EQ)
-    THEN IMP_RES_TAC LESS_CASES_IMP
-    THEN RW_TAC bool_ss [SUB_RIGHT_ADD]
-    THEN PROVE_TAC [GSYM NOT_LESS_EQUAL]);
+    \\ SIMP_TAC bool_ss [DIV_MULT_LESS_EQ,MOD_2EXP_LEM,SLICE_LEM1,
+         RIGHT_SUB_DISTRIB,SUB_SUB,SUB_LESS_EQ]
+    \\ Cases_on `n = n DIV 2 ** x * 2 ** x`
+    >> POP_ASSUM (fn th => SIMP_TAC arith_ss [SYM th])
+    \\ ASSUME_TAC (REWRITE_RULE [GSYM NOT_LESS] DIV_MULT_LESS_EQ)
+    \\ IMP_RES_TAC LESS_CASES_IMP
+    \\ RW_TAC bool_ss [SUB_RIGHT_ADD]
+    \\ PROVE_TAC [GSYM NOT_LESS_EQUAL]);
 
 val SLICE_LEM3 = prove(
   `!n h l. l < h ==> n MOD 2 ** SUC l <= n MOD 2 ** h`,
-  REPEAT STRIP_TAC THEN IMP_RES_TAC LESS_ADD_1
-    THEN POP_ASSUM (fn th => REWRITE_TAC [th])
-    THEN REWRITE_TAC [GSYM ADD1,GSYM ADD_SUC,GSYM (CONJUNCT2 ADD)]
-    THEN SIMP_TAC arith_ss [SLICE_LEM2]);
+  REPEAT STRIP_TAC \\ IMP_RES_TAC LESS_ADD_1
+    \\ POP_ASSUM (fn th => REWRITE_TAC [th])
+    \\ REWRITE_TAC [GSYM ADD1,GSYM ADD_SUC,GSYM (CONJUNCT2 ADD)]
+    \\ SIMP_TAC arith_ss [SLICE_LEM2]);
 
 val SLICE_THM = store_thm("SLICE_THM",
   `!n h l. SLICE h l n = BITS h l n * 2 ** l`,
   REPEAT STRIP_TAC
-    THEN REWRITE_TAC [SLICE_def,BITS_def,MOD_2EXP_def,DIV_2EXP_def]
-    THEN Cases_on `h < l`
-    THENL [
+    \\ REWRITE_TAC [SLICE_def,BITS_def,MOD_2EXP_def,DIV_2EXP_def]
+    \\ Cases_on `h < l`
+    << [
       IMP_RES_TAC SLICE_LEM3
-        THEN POP_ASSUM (fn th => ASSUME_TAC (SPEC `n` th))
-        THEN IMP_RES_TAC LESS_OR
-        THEN IMP_RES_TAC SUB_EQ_0
-        THEN ASM_SIMP_TAC arith_ss [EXP,MOD_1,MULT_CLAUSES],
-      REWRITE_TAC [DIV_MOD_MOD_DIV2]
-        THEN RULE_ASSUM_TAC (REWRITE_RULE [NOT_LESS])
-        THEN SUBST_OCCS_TAC
-               [([1],SPECL [`l`,`n MOD 2 ** SUC h`] TWOEXP_DIVISION)]
-        THEN IMP_RES_TAC LESS_EQUAL_ADD
-        THEN POP_ASSUM (fn th => SUBST_OCCS_TAC [([2],th)])
-        THEN SIMP_TAC bool_ss [ADD_SUC,ADD_SUB,MOD_MULT_MOD,
-               ZERO_LT_TWOEXP,EXP_ADD]]);
+        \\ POP_ASSUM (fn th => ASSUME_TAC (SPEC `n` th))
+        \\ IMP_RES_TAC LESS_OR
+        \\ IMP_RES_TAC SUB_EQ_0
+        \\ ASM_SIMP_TAC arith_ss [EXP,MOD_1,MULT_CLAUSES],
+      REWRITE_TAC [DIV_MOD_MOD_DIV3]
+        \\ RULE_ASSUM_TAC (REWRITE_RULE [NOT_LESS])
+        \\ SUBST_OCCS_TAC
+             [([1],SPECL [`l`,`n MOD 2 ** SUC h`] TWOEXP_DIVISION)]
+        \\ IMP_RES_TAC LESS_EQUAL_ADD
+        \\ POP_ASSUM (fn th => SUBST_OCCS_TAC [([2],th)])
+        \\ SIMP_TAC bool_ss [ADD_SUC,ADD_SUB,MOD_MULT_MOD,
+             ZERO_LT_TWOEXP,EXP_ADD]]);
 
 val SLICELT_THM = store_thm("SLICELT_THM",
   `!h l n. SLICE h l n < 2 ** SUC h`,
-  REPEAT STRIP_TAC THEN ASSUME_TAC (SPECL [`SUC h`,`n`] MOD_2EXP_LT)
-    THEN RW_TAC arith_ss [SLICE_def,MOD_2EXP_def,ZERO_LT_TWOEXP,SUB_RIGHT_LESS]);
+  REPEAT STRIP_TAC \\ ASSUME_TAC (SPECL [`SUC h`,`n`] MOD_2EXP_LT)
+    \\ RW_TAC arith_ss [SLICE_def,MOD_2EXP_def,ZERO_LT_TWOEXP,SUB_RIGHT_LESS]);
 
 val BITS_SLICE_THM = store_thm("BITS_SLICE_THM",
   `!h l n. BITS h l (SLICE h l n) = BITS h l n`,
@@ -436,13 +429,13 @@ val BITS_SLICE_THM = store_thm("BITS_SLICE_THM",
 
 val BITS_SLICE_THM2 = store_thm("BITS_SLICE_THM2",
   `!h l n. h <= h2 ==> (BITS h2 l (SLICE h l n) = BITS h l n)`,
-  REPEAT STRIP_TAC THEN LEFT_REWRITE_TAC [BITS_THM]
-    THEN SIMP_TAC bool_ss [SLICE_THM,ZERO_LT_TWOEXP,MULT_DIV]
-    THEN `SUC h - l <= SUC h2 - l` by DECIDE_TAC
-    THEN IMP_RES_TAC TWOEXP_MONO2 THEN POP_LAST_TAC
-    THEN ASSUME_TAC (SPECL [`h`,`l`,`n`] BITSLT_THM)
-    THEN IMP_RES_TAC LESS_LESS_EQ_TRANS
-    THEN ASM_SIMP_TAC bool_ss [LESS_MOD]);
+  REPEAT STRIP_TAC \\ LEFT_REWRITE_TAC [BITS_THM]
+    \\ SIMP_TAC bool_ss [SLICE_THM,ZERO_LT_TWOEXP,MULT_DIV]
+    \\ `SUC h - l <= SUC h2 - l` by DECIDE_TAC
+    \\ IMP_RES_TAC TWOEXP_MONO2 \\ POP_LAST_TAC
+    \\ ASSUME_TAC (SPECL [`h`,`l`,`n`] BITSLT_THM)
+    \\ IMP_RES_TAC LESS_LESS_EQ_TRANS
+    \\ ASM_SIMP_TAC bool_ss [LESS_MOD]);
 
 val SLICE_ZERO_THM = save_thm("SLICE_ZERO_THM",
   (GEN_ALL o REWRITE_RULE [MULT_RIGHT_1,EXP] o
@@ -450,8 +443,8 @@ val SLICE_ZERO_THM = save_thm("SLICE_ZERO_THM",
 
 val MOD_2EXP_MONO = store_thm("MOD_2EXP_MONO",
   `!n h l. l <= h ==> n MOD 2 ** l <= n MOD 2 ** SUC h`,
-  REPEAT STRIP_TAC THEN IMP_RES_TAC LESS_EQ_EXISTS
-    THEN ASM_SIMP_TAC arith_ss [SUC_ADD_SYM,SLICE_LEM2]);
+  REPEAT STRIP_TAC \\ IMP_RES_TAC LESS_EQ_EXISTS
+    \\ ASM_SIMP_TAC arith_ss [SUC_ADD_SYM,SLICE_LEM2]);
 
 val SLICE_COMP_THM = store_thm("SLICE_COMP_THM",
   `!h m l n. (SUC m) <= h /\ l <= m ==>
@@ -482,10 +475,10 @@ val BITS_SUM2 = store_thm("BITS_SUM2",
 val SLICE_TWOEXP = prove(
   `!h l a n. SLICE (h + n) (l + n) (a * 2 ** n) = (SLICE h l a) * 2 ** n`,
   REPEAT STRIP_TAC
-    THEN SUBST1_TAC (SPECL [`l`,`n`] ADD_COMM)
-    THEN RW_TAC bool_ss [(GSYM o CONJUNCT2) ADD,SLICE_THM,BITS_THM,
-           MULT_DIV,EXP_ADD,GSYM DIV_DIV_DIV_MULT,ZERO_LT_TWOEXP]
-    THEN SIMP_TAC arith_ss [AC MULT_ASSOC MULT_COMM]);
+    \\ SUBST1_TAC (SPECL [`l`,`n`] ADD_COMM)
+    \\ RW_TAC bool_ss [(GSYM o CONJUNCT2) ADD,SLICE_THM,BITS_THM,
+         MULT_DIV,EXP_ADD,GSYM DIV_DIV_DIV_MULT,ZERO_LT_TWOEXP]
+    \\ SIMP_TAC arith_ss [AC MULT_ASSOC MULT_COMM]);
  
 val SPEC_SLICE_TWOEXP =
   (GEN_ALL o SIMP_RULE arith_ss [] o DISCH `n <= l /\ n <= h` o
@@ -496,13 +489,13 @@ val SLICE_COMP_THM2 = store_thm("SLICE_COMP_THM2",
       h <= x /\ y <= l ==>
         (SLICE h l (SLICE x y n) = SLICE h l n)`,
   REPEAT STRIP_TAC
-    THEN Cases_on `h < l` THEN1 ASM_SIMP_TAC bool_ss [SLICE_ZERO]
-    THEN `y <= h` by DECIDE_TAC
-    THEN SUBST1_TAC (SPECL [`n`,`x`,`y`] SLICE_THM)
-    THEN ASM_SIMP_TAC bool_ss [SPEC_SLICE_TWOEXP]
-    THEN ASM_SIMP_TAC arith_ss [SLICE_THM,BITS_COMP_THM2,MIN_DEF]
-    THEN SIMP_TAC bool_ss [GSYM MULT_ASSOC,GSYM EXP_ADD]
-    THEN ASM_SIMP_TAC arith_ss []);
+    \\ Cases_on `h < l` >> ASM_SIMP_TAC bool_ss [SLICE_ZERO]
+    \\ `y <= h` by DECIDE_TAC
+    \\ SUBST1_TAC (SPECL [`n`,`x`,`y`] SLICE_THM)
+    \\ ASM_SIMP_TAC bool_ss [SPEC_SLICE_TWOEXP]
+    \\ ASM_SIMP_TAC arith_ss [SLICE_THM,BITS_COMP_THM2,MIN_DEF]
+    \\ SIMP_TAC bool_ss [GSYM MULT_ASSOC,GSYM EXP_ADD]
+    \\ ASM_SIMP_TAC arith_ss []);
 
 (* ------------------------------------------------------------------------- *)
 
@@ -512,8 +505,8 @@ val lem2 = prove(`!a b c. a * (b * c) = a * c * b`,
 
 val lem3 = prove(
   `!a m n. n <= m ==> (a * 2 ** m DIV 2 ** n = a * 2 ** (m - n))`,
-  REPEAT STRIP_TAC THEN IMP_RES_TAC LESS_EQUAL_ADD
-    THEN ASM_SIMP_TAC arith_ss [EXP_ADD,MULT_DIV,ZERO_LT_TWOEXP,lem2]);
+  REPEAT STRIP_TAC \\ IMP_RES_TAC LESS_EQUAL_ADD
+    \\ ASM_SIMP_TAC arith_ss [EXP_ADD,MULT_DIV,ZERO_LT_TWOEXP,lem2]);
 
 (* |- !a m n. n < m ==> (a * 2 ** m DIV 2 ** n = a * 2 ** (m - n)) *)
 val lem4 = SIMP_PROVE std_ss [LESS_IMP_LESS_OR_EQ,lem3]
@@ -523,19 +516,20 @@ val BIT_COMP_THM3 = store_thm("BIT_COMP_THM3",
   `!h m l n.  SUC m <= h /\ l <= m ==>
          (BITS h (SUC m) n * 2 ** (SUC m - l) + BITS m l n = BITS h l n)`,
   REPEAT STRIP_TAC
-    THEN IMP_RES_TAC (REWRITE_RULE [SLICE_THM] SLICE_COMP_THM)
-    THEN POP_LAST_TAC
-    THEN POP_ASSUM (fn th => ASSUME_TAC (GEN `l'`
-           (MATCH_MP (SPEC `2 ** l` lem) (SPEC `n` th))))
-    THEN POP_ASSUM (fn th => ASSUME_TAC
-           (ONCE_REWRITE_RULE [ADD_COMM] (SPEC `l` th)))
-    THEN `l < SUC m` by ASM_SIMP_TAC arith_ss []
-    THEN FULL_SIMP_TAC arith_ss [lem4,ADD_DIV_ADD_DIV,MULT_DIV,ZERO_LT_TWOEXP]);
+    \\ IMP_RES_TAC (REWRITE_RULE [SLICE_THM] SLICE_COMP_THM)
+    \\ POP_LAST_TAC
+    \\ POP_ASSUM (fn th => ASSUME_TAC (GEN `l'`
+         (MATCH_MP (SPEC `2 ** l` lem) (SPEC `n` th))))
+    \\ POP_ASSUM (fn th => ASSUME_TAC
+         (ONCE_REWRITE_RULE [ADD_COMM] (SPEC `l` th)))
+    \\ `l < SUC m` by ASM_SIMP_TAC arith_ss []
+    \\ FULL_SIMP_TAC arith_ss [lem4,ADD_DIV_ADD_DIV,MULT_DIV,ZERO_LT_TWOEXP]);
 
 (* ------------------------------------------------------------------------- *)
 
 val BITS_SUM = store_thm("BITS_SUM",
-  `!h l a b. b < 2 ** l ==> (BITS h l (a * 2 ** l + b) = BITS h l (a * 2 ** l))`,
+  `!h l a b. b < 2 ** l ==>
+      (BITS h l (a * 2 ** l + b) = BITS h l (a * 2 ** l))`,
   RW_TAC bool_ss [BITS_THM,DIV_MULT,MULT_DIV,ZERO_LT_TWOEXP]);
  
 val BITS_SUM2 = store_thm("BITS_SUM2",
@@ -545,10 +539,10 @@ val BITS_SUM2 = store_thm("BITS_SUM2",
 val SLICE_TWOEXP = prove(
   `!h l a n. SLICE (h + n) (l + n) (a * 2 ** n) = (SLICE h l a) * 2 ** n`,
   REPEAT STRIP_TAC
-    THEN SUBST1_TAC (SPECL [`l`,`n`] ADD_COMM)
-    THEN RW_TAC bool_ss [(GSYM o CONJUNCT2) ADD,SLICE_THM,BITS_THM,MULT_DIV,
-           EXP_ADD,GSYM DIV_DIV_DIV_MULT,ZERO_LT_TWOEXP]
-    THEN SIMP_TAC arith_ss [AC MULT_ASSOC MULT_COMM]);
+    \\ SUBST1_TAC (SPECL [`l`,`n`] ADD_COMM)
+    \\ RW_TAC bool_ss [(GSYM o CONJUNCT2) ADD,SLICE_THM,BITS_THM,MULT_DIV,
+         EXP_ADD,GSYM DIV_DIV_DIV_MULT,ZERO_LT_TWOEXP]
+    \\ SIMP_TAC arith_ss [AC MULT_ASSOC MULT_COMM]);
  
 val SPEC_SLICE_TWOEXP =
   (GEN_ALL o SIMP_RULE arith_ss [] o DISCH `n <= l /\ n <= h` o
@@ -558,13 +552,13 @@ val SLICE_COMP_THM2 = store_thm("SLICE_COMP_THM2",
   `!h l x y n.  h <= x /\ y <= l ==>
         (SLICE h l (SLICE x y n) = SLICE h l n)`,
   REPEAT STRIP_TAC
-    THEN Cases_on `h < l` THEN1 ASM_SIMP_TAC bool_ss [SLICE_ZERO]
-    THEN `y <= h` by DECIDE_TAC
-    THEN SUBST1_TAC (SPECL [`n`,`x`,`y`] SLICE_THM)
-    THEN ASM_SIMP_TAC bool_ss [SPEC_SLICE_TWOEXP]
-    THEN ASM_SIMP_TAC arith_ss [SLICE_THM,BITS_COMP_THM2,MIN_DEF]
-    THEN SIMP_TAC bool_ss [GSYM MULT_ASSOC,GSYM EXP_ADD]
-    THEN ASM_SIMP_TAC arith_ss []);
+    \\ Cases_on `h < l` >> ASM_SIMP_TAC bool_ss [SLICE_ZERO]
+    \\ `y <= h` by DECIDE_TAC
+    \\ SUBST1_TAC (SPECL [`n`,`x`,`y`] SLICE_THM)
+    \\ ASM_SIMP_TAC bool_ss [SPEC_SLICE_TWOEXP]
+    \\ ASM_SIMP_TAC arith_ss [SLICE_THM,BITS_COMP_THM2,MIN_DEF]
+    \\ SIMP_TAC bool_ss [GSYM MULT_ASSOC,GSYM EXP_ADD]
+    \\ ASM_SIMP_TAC arith_ss []);
 
 (* ------------------------------------------------------------------------- *)
 
@@ -582,19 +576,17 @@ val NOT_BITS2 = store_thm("NOT_BITS2",
 
 val BIT_SLICE = store_thm("BIT_SLICE",
   `!n a b. (BIT n a = BIT n b) = (SLICE n n a = SLICE n n b)`,
-  REPEAT STRIP_TAC THEN EQ_TAC
-    THENL [
-      Cases_on `BIT n a`
-        THEN FULL_SIMP_TAC arith_ss [BIT_def,SLICE_THM,NOT_BITS2],
-      Cases_on `BITS n n a = 1`
-        THEN Cases_on `BITS n n b = 1`
-        THEN FULL_SIMP_TAC arith_ss [BIT_def,SLICE_THM,NOT_BITS2,MULT_CLAUSES,
-               REWRITE_RULE [GSYM NOT_ZERO_LT_ZERO] ZERO_LT_TWOEXP]]);
+  REPEAT STRIP_TAC \\ EQ_TAC
+    >> (Cases_on `BIT n a` \\
+        FULL_SIMP_TAC arith_ss [BIT_def,SLICE_THM,NOT_BITS2])
+    \\ Cases_on `BITS n n a = 1` \\ Cases_on `BITS n n b = 1`
+    \\ FULL_SIMP_TAC arith_ss [BIT_def,SLICE_THM,NOT_BITS2,MULT_CLAUSES,
+         REWRITE_RULE [GSYM NOT_ZERO_LT_ZERO] ZERO_LT_TWOEXP]);
 
 val BIT_SLICE_LEM = store_thm("BIT_SLICE_LEM",
   `!y x n. SBIT (BIT x n) (x + y) = (SLICE x x n) * 2 ** y`,
   RW_TAC arith_ss [SBIT_def,BIT_SLICE,SLICE_THM,BIT_def,EXP_ADD]
-    THEN FULL_SIMP_TAC bool_ss [GSYM NOT_BITS]);
+    \\ FULL_SIMP_TAC bool_ss [GSYM NOT_BITS]);
 
 (* |- !x n. SBIT (BIT x n) x = SLICE x x n *)
 val BIT_SLICE_THM = save_thm("BIT_SLICE_THM",
@@ -610,31 +602,31 @@ val BIT_SLICE_THM3 = store_thm("BIT_SLICE_THM3",
 
 val BIT_SLICE_THM4 = store_thm("BIT_SLICE_THM4",
   `!b h l n. BIT b (SLICE h l n) = l <= b /\ b <= h /\ BIT b n`,
-  REPEAT STRIP_TAC THEN Cases_on `l <= b /\ b <= h`
-    THEN RW_TAC arith_ss [BIT_SLICE_THM2,SLICE_COMP_THM2]
-    THEN REWRITE_TAC [GSYM BIT_SLICE_THM2]
-    THEN FULL_SIMP_TAC arith_ss [SLICE_THM,BIT_def,NOT_LESS_EQUAL,
-           SPECL [`b`,`b`] BITS_THM,SUC_SUB,NOT_MOD2_LEM2]
-    THENL [
+  REPEAT STRIP_TAC \\ Cases_on `l <= b /\ b <= h`
+    \\ RW_TAC arith_ss [BIT_SLICE_THM2,SLICE_COMP_THM2]
+    \\ REWRITE_TAC [GSYM BIT_SLICE_THM2]
+    \\ FULL_SIMP_TAC arith_ss [SLICE_THM,BIT_def,NOT_LESS_EQUAL,
+         SPECL [`b`,`b`] BITS_THM,SUC_SUB,NOT_MOD2_LEM2]
+    << [
       IMP_RES_TAC LESS_ADD_1
-        THEN ASM_SIMP_TAC arith_ss [MULT_ASSOC,MULT_DIV,ZERO_LT_TWOEXP,
-               ONCE_REWRITE_RULE [ADD_COMM] EXP_ADD]
-        THEN METIS_TAC [MOD_EQ_0,DECIDE ``0 < 2``,MULT_ASSOC,MULT_COMM],
+        \\ ASM_SIMP_TAC arith_ss [MULT_ASSOC,MULT_DIV,ZERO_LT_TWOEXP,
+             ONCE_REWRITE_RULE [ADD_COMM] EXP_ADD]
+        \\ METIS_TAC [MOD_EQ_0,DECIDE ``0 < 2``,MULT_ASSOC,MULT_COMM],
       `SUC h <= b` by DECIDE_TAC
-        THEN `BITS h l n * 2 ** l < 2 ** b` by METIS_TAC [TWOEXP_MONO2,
-               GSYM SLICE_THM,SLICELT_THM,LESS_LESS_EQ_TRANS]
-        THEN ASM_SIMP_TAC std_ss [LESS_DIV_EQ_ZERO]]);
+        \\ `BITS h l n * 2 ** l < 2 ** b` by METIS_TAC [TWOEXP_MONO2,
+             GSYM SLICE_THM,SLICELT_THM,LESS_LESS_EQ_TRANS]
+        \\ ASM_SIMP_TAC std_ss [LESS_DIV_EQ_ZERO]]);
 
 val SUB_BITS = prove(
   `!h l a b. (BITS (SUC h) l a = BITS (SUC h) l b) ==>
       (BITS h l a = BITS h l b)`,
   REPEAT STRIP_TAC
-    THEN Cases_on `h < l` THEN1 RW_TAC bool_ss [BITS_ZERO]
-    THEN RULE_ASSUM_TAC (REWRITE_RULE [NOT_LESS])
-    THEN POP_ASSUM (fn th => ONCE_REWRITE_TAC
-           [(GSYM o SIMP_RULE arith_ss [th,SUB_ADD] o
-             SPECL [`SUC h`,`l`,`h - l`,`0`]) BITS_COMP_THM])
-    THEN ASM_REWRITE_TAC []);
+    \\ Cases_on `h < l` >> RW_TAC bool_ss [BITS_ZERO]
+    \\ RULE_ASSUM_TAC (REWRITE_RULE [NOT_LESS])
+    \\ POP_ASSUM (fn th => ONCE_REWRITE_TAC
+         [(GSYM o SIMP_RULE arith_ss [th,SUB_ADD] o
+           SPECL [`SUC h`,`l`,`h - l`,`0`]) BITS_COMP_THM])
+    \\ ASM_REWRITE_TAC []);
 
 val SBIT_DIV = store_thm("SBIT_DIV",
   `!b m n. n < m ==> (SBIT b (m - n) = SBIT b m DIV 2 ** n)`,
@@ -645,14 +637,14 @@ val BITS_SUC = store_thm("BITS_SUC",
   `!h l n.  l <= SUC h ==>
      (SBIT (BIT (SUC h) n) (SUC h - l) + BITS h l n = BITS (SUC h) l n)`,
   REPEAT STRIP_TAC
-    THEN Cases_on `l = SUC h`
-    THENL [
+    \\ Cases_on `l = SUC h`
+    << [
       RW_TAC arith_ss [EXP,BITS_ZERO,SBIT_def,BIT_def]
-        THEN FULL_SIMP_TAC bool_ss [NOT_BITS2],
+        \\ FULL_SIMP_TAC bool_ss [NOT_BITS2],
       `l <= h` by ASM_SIMP_TAC arith_ss []
-        THEN IMP_RES_TAC LESS_EQ_IMP_LESS_SUC
-        THEN ASM_SIMP_TAC arith_ss [SBIT_DIV,BIT_SLICE_THM,SLICE_THM,
-               lem4,SPECL [`SUC h`,`h`] BIT_COMP_THM3]]);
+        \\ IMP_RES_TAC LESS_EQ_IMP_LESS_SUC
+        \\ ASM_SIMP_TAC arith_ss [SBIT_DIV,BIT_SLICE_THM,SLICE_THM,
+             lem4,SPECL [`SUC h`,`h`] BIT_COMP_THM3]]);
 
 val BITS_SUC_THM = store_thm("BITS_SUC_THM",
   `!h l n. BITS (SUC h) l n =
@@ -668,113 +660,117 @@ val BIT_BITS_LEM = prove(
   `!h l a b. l <= h ==> (BITS h l a = BITS h l b) ==>
       (BIT h a = BIT h b)`,
   RW_TAC bool_ss [BIT_SLICE,SLICE_THM]
-    THEN PAT_ASSUM `l <= h` (fn th => ONCE_REWRITE_TAC
-           [(GSYM o SIMP_RULE arith_ss [th,SUB_ADD] o
-             SPECL [`h`,`l`,`h - l`,`h - l`]) BITS_COMP_THM])
-    THEN ASM_REWRITE_TAC []);
+    \\ PAT_ASSUM `l <= h` (fn th => ONCE_REWRITE_TAC
+         [(GSYM o SIMP_RULE arith_ss [th,SUB_ADD] o
+           SPECL [`h`,`l`,`h - l`,`h - l`]) BITS_COMP_THM])
+    \\ ASM_REWRITE_TAC []);
 
 val BIT_BITS_THM = store_thm("BIT_BITS_THM",
   `!h l a b. (!x. l <= x /\ x <= h ==>
       (BIT x a = BIT x b)) = (BITS h l a = BITS h l b)`,
-  Induct_on `h` THEN REPEAT STRIP_TAC
-    THENL [
-      Cases_on `l = 0`
-        THEN RW_TAC arith_ss [BIT_SLICE,SLICE_THM,EXP,
-               SPEC `0` BITS_ZERO,NOT_ZERO_LT_ZERO],
-      EQ_TAC THEN REPEAT STRIP_TAC
-        THENL [
-          RW_TAC bool_ss [BITS_SUC_THM]
-            THEN RULE_ASSUM_TAC (REWRITE_RULE [NOT_LESS])
-            THEN PAT_ASSUM `!x. l <= x /\ x <= SUC h ==> (BIT x a = BIT x b)`
-                   (fn th => ASM_SIMP_TAC bool_ss
-                      [SIMP_RULE arith_ss [] (SPEC `SUC h` th)]
-                       THEN ASSUME_TAC (MATCH_MP ((BETA_RULE o
-                         SPECL [`\x. BIT x a = BIT x b`,`l`,`h`]) DECEND_LEMMA) th))
-            THEN FIRST_ASSUM (fn th => ASSUME_TAC (SPECL [`l`,`a`,`b`] th))
-            THEN FULL_SIMP_TAC bool_ss [],
-          IMP_RES_TAC SUB_BITS
-            THEN FIRST_ASSUM (fn th => RULE_ASSUM_TAC
-                   (REWRITE_RULE [SYM (SPECL [`l`,`a`,`b`] th)]))
-            THEN Cases_on `x <= h` THEN ASM_SIMP_TAC bool_ss []
-            THEN `x = SUC h` by ASM_SIMP_TAC arith_ss []
-            THEN Cases_on `l = SUC h` THEN1 FULL_SIMP_TAC bool_ss [BIT_def]
-            THEN `l <= SUC h` by ASM_SIMP_TAC arith_ss []
-            THEN POP_ASSUM (fn th => ASSUME_TAC
-                   (SIMP_RULE bool_ss [th] (SPECL [`SUC h`,`l`,`a`,`b`] BIT_BITS_LEM)))
-            THEN FULL_SIMP_TAC bool_ss []]]);
+  Induct_on `h` \\ REPEAT STRIP_TAC
+    >> (Cases_on `l = 0` \\ RW_TAC arith_ss [BIT_SLICE,SLICE_THM,EXP,
+          SPEC `0` BITS_ZERO,NOT_ZERO_LT_ZERO])
+    \\ EQ_TAC \\ REPEAT STRIP_TAC
+    << [
+      RW_TAC bool_ss [BITS_SUC_THM]
+        \\ RULE_ASSUM_TAC (REWRITE_RULE [NOT_LESS])
+        \\ PAT_ASSUM `!x. l <= x /\ x <= SUC h ==> (BIT x a = BIT x b)`
+             (fn th => ASM_SIMP_TAC bool_ss
+                       [SIMP_RULE arith_ss [] (SPEC `SUC h` th)] \\
+                     ASSUME_TAC (MATCH_MP ((BETA_RULE o SPECL
+                       [`\x. BIT x a = BIT x b`,`l`,`h`]) DECEND_LEMMA) th))
+        \\ FIRST_ASSUM (fn th => ASSUME_TAC (SPECL [`l`,`a`,`b`] th))
+        \\ FULL_SIMP_TAC bool_ss [],
+      IMP_RES_TAC SUB_BITS
+        \\ FIRST_ASSUM (fn th => RULE_ASSUM_TAC
+             (REWRITE_RULE [SYM (SPECL [`l`,`a`,`b`] th)]))
+        \\ Cases_on `x <= h` \\ ASM_SIMP_TAC bool_ss []
+        \\ `x = SUC h` by ASM_SIMP_TAC arith_ss []
+        \\ Cases_on `l = SUC h` >> FULL_SIMP_TAC bool_ss [BIT_def]
+        \\ `l <= SUC h` by ASM_SIMP_TAC arith_ss []
+        \\ POP_ASSUM (fn th => ASSUME_TAC (SIMP_RULE bool_ss [th]
+             (SPECL [`SUC h`,`l`,`a`,`b`] BIT_BITS_LEM)))
+        \\ FULL_SIMP_TAC bool_ss []]);
 
 (* ------------------------------------------------------------------------- *)
+
+val LSB_ODD = store_thm("LSB_ODD", `LSB = ODD`,
+  ONCE_REWRITE_TAC [FUN_EQ_THM]
+    \\ SIMP_TAC arith_ss [ODD_MOD2_LEM,LSB_def,BIT_def,BITS_THM2,EXP,DIV_1]);
 
 val BITV_THM = store_thm("BITV_THM",
   `!b n. BITV n b = SBIT (BIT b n) 0`,
   RW_TAC arith_ss [BITV_def,BIT_def,SBIT_def]
-    THEN FULL_SIMP_TAC bool_ss [NOT_BITS2]);
+    \\ FULL_SIMP_TAC bool_ss [NOT_BITS2]);
 
 (* ------------------------------------------------------------------------- *)
 
 val BITWISE_LT_2EXP = store_thm("BITWISE_LT_2EXP",
   `!n op a b. BITWISE n op a b < 2 ** n`,
   Induct_on `n`
-    THEN RW_TAC bool_ss [ADD_0,TIMES2,LESS_IMP_LESS_ADD,LESS_MONO_ADD,
-           BITWISE_def,SBIT_def,EXP]
-    THEN REDUCE_TAC);
+    \\ RW_TAC bool_ss [ADD_0,TIMES2,LESS_IMP_LESS_ADD,LESS_MONO_ADD,
+         BITWISE_def,SBIT_def,EXP]
+    \\ REDUCE_TAC);
 
 val LESS_EXP_MULT2 = prove(
   `!a b. a < b ==> ?p. 2 ** b = 2 ** (p + 1) * 2 ** a`,
   REPEAT STRIP_TAC
-    THEN IMP_RES_TAC LESS_ADD_1
-    THEN RULE_ASSUM_TAC (ONCE_REWRITE_RULE [SIMP_RULE arith_ss []
+    \\ IMP_RES_TAC LESS_ADD_1
+    \\ RULE_ASSUM_TAC (ONCE_REWRITE_RULE [SIMP_RULE arith_ss []
            (SPEC `2` (GSYM EXP_INJECTIVE))])
-    THEN EXISTS_TAC `p` THEN FULL_SIMP_TAC arith_ss [EXP_ADD,MULT_COMM]);
+    \\ EXISTS_TAC `p` \\ FULL_SIMP_TAC arith_ss [EXP_ADD,MULT_COMM]);
 
 val BITWISE_LEM = prove(
   `!n op a b. BIT n (BITWISE (SUC n) op a b) = op (BIT n a) (BIT n b)`,
   RW_TAC arith_ss [SBIT_def,BITWISE_def,NOT_BIT]
-    THEN1 SIMP_TAC arith_ss [BIT_def,BITS_THM,SUC_SUB,
-            REWRITE_RULE [BITWISE_LT_2EXP]
-              (SPECL [`BITWISE n op a b`,`2 ** n`] DIV_MULT_1)]
-    THEN SIMP_TAC arith_ss [BITS_THM,LESS_DIV_EQ_ZERO,BITWISE_LT_2EXP,SUC_SUB]);
+    >> SIMP_TAC arith_ss [BIT_def,BITS_THM,SUC_SUB,
+         REWRITE_RULE [BITWISE_LT_2EXP]
+           (SPECL [`BITWISE n op a b`,`2 ** n`] DIV_MULT_1)]
+    \\ SIMP_TAC arith_ss [BITS_THM,LESS_DIV_EQ_ZERO,BITWISE_LT_2EXP,SUC_SUB]);
 
-val TWO_SUC_SUB = GEN_ALL (SIMP_CONV bool_ss [SUC_SUB,EXP_1] ``2 ** (SUC x - x)``);
+val TWO_SUC_SUB =
+  GEN_ALL (SIMP_CONV bool_ss [SUC_SUB,EXP_1] ``2 ** (SUC x - x)``);
 
 val BITWISE_THM = store_thm("BITWISE_THM",
   `!x n op a b. x < n ==> (BIT x (BITWISE n op a b) = op (BIT x a) (BIT x b))`,
   Induct_on `n`
-    THEN REPEAT STRIP_TAC THEN1 FULL_SIMP_TAC arith_ss []
-    THEN Cases_on `x = n` THEN1 ASM_REWRITE_TAC [BITWISE_LEM]
-    THEN `x < n` by ASM_SIMP_TAC arith_ss []
-    THEN RW_TAC arith_ss [BITWISE_def,SBIT_def]
-    THEN LEFT_REWRITE_TAC [BIT_def]
-    THEN ASM_REWRITE_TAC [BITS_THM]
-    THEN IMP_RES_TAC LESS_EXP_MULT2 THEN POP_LAST_TAC
-    THEN ASM_SIMP_TAC bool_ss [ZERO_LT_TWOEXP,ADD_DIV_ADD_DIV,
-           TWO_SUC_SUB,GSYM ADD1,EXP,ONCE_REWRITE_RULE [MULT_COMM]
-           (REWRITE_RULE [DECIDE (Term `0 < 2`)] (SPEC `2` MOD_TIMES))]
-    THEN SUBST_OCCS_TAC [([2],SYM (SPEC `x` TWO_SUC_SUB))]
-    THEN ASM_SIMP_TAC bool_ss [GSYM BITS_THM,GSYM BIT_def]);
+    \\ REPEAT STRIP_TAC >> FULL_SIMP_TAC arith_ss []
+    \\ Cases_on `x = n` >> ASM_REWRITE_TAC [BITWISE_LEM]
+    \\ `x < n` by ASM_SIMP_TAC arith_ss []
+    \\ RW_TAC arith_ss [BITWISE_def,SBIT_def]
+    \\ LEFT_REWRITE_TAC [BIT_def]
+    \\ ASM_REWRITE_TAC [BITS_THM]
+    \\ IMP_RES_TAC LESS_EXP_MULT2 \\ POP_LAST_TAC
+    \\ ASM_SIMP_TAC bool_ss [ZERO_LT_TWOEXP,ADD_DIV_ADD_DIV,
+         TWO_SUC_SUB,GSYM ADD1,EXP,ONCE_REWRITE_RULE [MULT_COMM]
+         (REWRITE_RULE [DECIDE (Term `0 < 2`)] (SPEC `2` MOD_TIMES))]
+    \\ SUBST_OCCS_TAC [([2],SYM (SPEC `x` TWO_SUC_SUB))]
+    \\ ASM_SIMP_TAC bool_ss [GSYM BITS_THM,GSYM BIT_def]);
 
 val BITWISE_COR = store_thm("BITWISE_COR",
   `!x n op a b. x < n ==> op (BIT x a) (BIT x b) ==>
       ((BITWISE n op a b DIV 2 ** x) MOD 2 = 1)`,
-  NTAC 6 STRIP_TAC THEN IMP_RES_TAC BITWISE_THM
-    THEN NTAC 2 (WEAKEN_TAC (K true))
-    THEN POP_ASSUM (fn th => REWRITE_TAC [GSYM th])
-    THEN ASM_REWRITE_TAC [BITS_THM,BIT_def,DIV_1,EXP_1,SUC_SUB]);
+  NTAC 6 STRIP_TAC \\ IMP_RES_TAC BITWISE_THM
+    \\ NTAC 2 (WEAKEN_TAC (K true))
+    \\ POP_ASSUM (fn th => REWRITE_TAC [GSYM th])
+    \\ ASM_REWRITE_TAC [BITS_THM,BIT_def,DIV_1,EXP_1,SUC_SUB]);
 
 val BITWISE_NOT_COR = store_thm("BITWISE_NOT_COR",
   `!x n op a b. x < n ==> ~op (BIT x a) (BIT x b) ==>
       ((BITWISE n op a b DIV 2 ** x) MOD 2 = 0)`,
-  NTAC 6 STRIP_TAC THEN IMP_RES_TAC BITWISE_THM
-    THEN NTAC 2 (WEAKEN_TAC (K true))
-    THEN POP_ASSUM (fn th => REWRITE_TAC [GSYM th])
-    THEN ASM_REWRITE_TAC [BITS_THM,BIT_def,GSYM NOT_MOD2_LEM,DIV_1,EXP_1,SUC_SUB]);
+  NTAC 6 STRIP_TAC \\ IMP_RES_TAC BITWISE_THM
+    \\ NTAC 2 (WEAKEN_TAC (K true))
+    \\ POP_ASSUM (fn th => REWRITE_TAC [GSYM th])
+    \\ ASM_REWRITE_TAC [BITS_THM,BIT_def,GSYM NOT_MOD2_LEM,DIV_1,EXP_1,SUC_SUB]
+);
 
 val BITWISE_BITS = store_thm("BITWISE_BITS",
   `!wl op a b. BITWISE (SUC wl) op (BITS wl 0 a) (BITS wl 0 b) =
                BITWISE (SUC wl) op a b`,
-  Induct THEN FULL_SIMP_TAC arith_ss [BITWISE_def,BIT_def,BITS_COMP_THM2,MIN_DEF]
-    THEN POP_ASSUM (fn th => ONCE_REWRITE_TAC [GSYM th])
-    THEN SIMP_TAC arith_ss [BITS_COMP_THM2,MIN_DEF]);
+  Induct \\ FULL_SIMP_TAC arith_ss [BITWISE_def,BIT_def,BITS_COMP_THM2,MIN_DEF]
+    \\ POP_ASSUM (fn th => ONCE_REWRITE_TAC [GSYM th])
+    \\ SIMP_TAC arith_ss [BITS_COMP_THM2,MIN_DEF]);
 
 (* ------------------------------------------------------------------------- *)
 
@@ -790,17 +786,17 @@ val lem2 = MATCH_MP lem (REWRITE_RULE [SUB_0] (SPECL [`n`,`0`,`a`] BITSLT_THM));
 
 val BITWISE_ONE_COMP_LEM = store_thm("BITWISE_ONE_COMP_LEM",
   `!n a b. BITWISE (SUC n) (\x y. ~x) a b = 2 ** (SUC n) - 1 - BITS n 0 a`,
-  Induct_on `n` THEN REPEAT STRIP_TAC
-    THEN1 RW_TAC arith_ss [SBIT_def,BIT_def,BITWISE_def,NOT_BITS2]
-    THEN RW_TAC arith_ss [BITWISE_def,SBIT_def,REWRITE_RULE [SLICE_THM] BITS_SUC2]
-    THEN RULE_ASSUM_TAC (SIMP_RULE bool_ss [NOT_BIT,NOT_BITS,BIT_def])
-    THEN ASM_SIMP_TAC arith_ss [MULT_CLAUSES]
-    THENL [
+  Induct_on `n` \\ REPEAT STRIP_TAC
+    >> RW_TAC arith_ss [SBIT_def,BIT_def,BITWISE_def,NOT_BITS2]
+    \\ RW_TAC arith_ss [BITWISE_def,SBIT_def,REWRITE_RULE [SLICE_THM] BITS_SUC2]
+    \\ RULE_ASSUM_TAC (SIMP_RULE bool_ss [NOT_BIT,NOT_BITS,BIT_def])
+    \\ ASM_SIMP_TAC arith_ss [MULT_CLAUSES]
+    << [
       Cases_on `2 ** SUC n = BITS n 0 a + 1`
-        THEN1 ASM_SIMP_TAC arith_ss [SUB_RIGHT_ADD,EXP]
-        THEN ASSUME_TAC lem2
-        THEN `~(2 ** SUC n <= BITS n 0 a + 1)` by ASM_SIMP_TAC arith_ss []
-        THEN ASM_SIMP_TAC arith_ss [SUB_RIGHT_ADD,EXP],
+        >> ASM_SIMP_TAC arith_ss [SUB_RIGHT_ADD,EXP]
+        \\ ASSUME_TAC lem2
+        \\ `~(2 ** SUC n <= BITS n 0 a + 1)` by ASM_SIMP_TAC arith_ss []
+        \\ ASM_SIMP_TAC arith_ss [SUB_RIGHT_ADD,EXP],
       REWRITE_TAC [REWRITE_CONV [ADD_SUB,TIMES2] (Term`2 * a - a`),SUB_PLUS,EXP]
     ]
 );
@@ -809,13 +805,13 @@ val BITWISE_ONE_COMP_LEM = store_thm("BITWISE_ONE_COMP_LEM",
 
 val BIT_SET_NOT_ZERO = prove(
   `!a. (a MOD 2 = 1) ==> (1 <= a)`,
-  SPOSE_NOT_THEN STRIP_ASSUME_TAC THEN `a = 0` by DECIDE_TAC
-    THEN FULL_SIMP_TAC arith_ss [ZERO_MOD]);
+  SPOSE_NOT_THEN STRIP_ASSUME_TAC \\ `a = 0` by DECIDE_TAC
+    \\ FULL_SIMP_TAC arith_ss [ZERO_MOD]);
  
 val BIT_SET_NOT_ZERO_COR = prove(
   `!x n op a b. x < n ==> op (BIT x a) (BIT x b) ==>
       (1 <= (BITWISE n op a b DIV 2 ** x))`,
-  REPEAT STRIP_TAC THEN ASM_SIMP_TAC bool_ss [BITWISE_COR,BIT_SET_NOT_ZERO]);
+  REPEAT STRIP_TAC \\ ASM_SIMP_TAC bool_ss [BITWISE_COR,BIT_SET_NOT_ZERO]);
  
 val BIT_SET_NOT_ZERO_COR2 =
   REWRITE_RULE [DIV_1,EXP] (SPEC `0` BIT_SET_NOT_ZERO_COR);
@@ -833,8 +829,8 @@ val SBIT_MULT = store_thm("SBIT_MULT",
 
 val lemma1 = prove(
   `!a b n. 0 < n ==> ((a + SBIT b n) DIV 2 = a DIV 2 + SBIT b (n - 1))`,
-  RW_TAC arith_ss [SBIT_def] THEN IMP_RES_TAC LESS_ADD_1
-    THEN FULL_SIMP_TAC arith_ss [GSYM ADD1,ADD_DIV_ADD_DIV2,EXP]);
+  RW_TAC arith_ss [SBIT_def] \\ IMP_RES_TAC LESS_ADD_1
+    \\ FULL_SIMP_TAC arith_ss [GSYM ADD1,ADD_DIV_ADD_DIV2,EXP]);
 
 val lemma2 = (ONCE_REWRITE_RULE [MULT_COMM] o REWRITE_RULE [EXP_1] o
               INST [`m` |-> `1`] o SPEC_ALL) SBIT_MULT;
@@ -842,36 +838,35 @@ val lemma2 = (ONCE_REWRITE_RULE [MULT_COMM] o REWRITE_RULE [EXP_1] o
 val lemma3 = prove(
   `!n op a b. 0 < n ==> (BITWISE n op a b MOD 2 = SBIT (op (LSB a) (LSB b)) 0)`,
   RW_TAC bool_ss [LSB_def]
-    THEN POP_ASSUM (fn th => ONCE_REWRITE_TAC
+    \\ POP_ASSUM (fn th => ONCE_REWRITE_TAC
            [MATCH_MP ((GSYM o SPEC `0`) BITWISE_THM) th])
-    THEN RW_TAC bool_ss [GSYM LSB_def,LSB_ODD,ODD_MOD2_LEM,SBIT_def,EXP]
-    THEN FULL_SIMP_TAC bool_ss [GSYM NOT_MOD2_LEM]);
+    \\ RW_TAC bool_ss [GSYM LSB_def,LSB_ODD,ODD_MOD2_LEM,SBIT_def,EXP]
+    \\ FULL_SIMP_TAC bool_ss [GSYM NOT_MOD2_LEM]);
  
 val lemma4 = prove(
   `!n op a b. 0 < n /\ BITWISE n op a b <= SBIT (op (LSB a) (LSB b)) 0 ==>
               (BITWISE n op a b = SBIT (op (LSB a) (LSB b)) 0)`,
   RW_TAC arith_ss [LSB_def,SBIT_def,EXP]
-    THEN IMP_RES_TAC BIT_SET_NOT_ZERO_COR2
-    THEN ASM_SIMP_TAC arith_ss []);
+    \\ IMP_RES_TAC BIT_SET_NOT_ZERO_COR2
+    \\ ASM_SIMP_TAC arith_ss []);
 
 val BITWISE_ISTEP = prove(
   `!n op a b. 0 < n ==>
       (BITWISE n op (a DIV 2) (b DIV 2) =
        (BITWISE n op a b) DIV 2 + SBIT (op (BIT n a) (BIT n b)) (n - 1))`,
-  Induct_on `n`
-    THEN REPEAT STRIP_TAC THEN1 FULL_SIMP_TAC arith_ss []
-    THEN Cases_on `n = 0` THEN1 RW_TAC arith_ss [BITWISE_def,SBIT_def,BIT_DIV2]
-    THEN FULL_SIMP_TAC bool_ss [NOT_ZERO_LT_ZERO,BITWISE_def,SUC_SUB1,BIT_DIV2,lemma1]
-);
+  Induct_on `n` \\ REPEAT STRIP_TAC >> FULL_SIMP_TAC arith_ss []
+    \\ Cases_on `n = 0` >> RW_TAC arith_ss [BITWISE_def,SBIT_def,BIT_DIV2]
+    \\ FULL_SIMP_TAC bool_ss
+         [NOT_ZERO_LT_ZERO,BITWISE_def,SUC_SUB1,BIT_DIV2,lemma1]);
  
 val BITWISE_EVAL = store_thm("BITWISE_EVAL",
   `!n op a b. BITWISE (SUC n) op a b =
       2 * (BITWISE n op (a DIV 2) (b DIV 2)) + SBIT (op (LSB a) (LSB b)) 0`,
-  REPEAT STRIP_TAC THEN Cases_on `n = 0`
-    THEN1 RW_TAC arith_ss [BITWISE_def,MULT_CLAUSES,LSB_def]
-    THEN FULL_SIMP_TAC arith_ss [BITWISE_def,NOT_ZERO_LT_ZERO,BITWISE_ISTEP,
+  REPEAT STRIP_TAC \\ Cases_on `n = 0`
+    >> RW_TAC arith_ss [BITWISE_def,MULT_CLAUSES,LSB_def]
+    \\ FULL_SIMP_TAC arith_ss [BITWISE_def,NOT_ZERO_LT_ZERO,BITWISE_ISTEP,
            DIV_MULT_THM2,LEFT_ADD_DISTRIB,SUB_ADD,lemma2,lemma3]
-    THEN RW_TAC arith_ss [SUB_RIGHT_ADD,lemma4]);
+    \\ RW_TAC arith_ss [SUB_RIGHT_ADD,lemma4]);
 
 (* ------------------------------------------------------------------------- *)
 
@@ -879,10 +874,10 @@ val MOD_PLUS_RIGHT = store_thm("MOD_PLUS_RIGHT",
  `!n. 0<n ==> !j k. ((j + (k MOD n)) MOD n) = ((j+k) MOD n)`,
    let fun SUBS th = SUBST_OCCS_TAC [([2],th)]
    in
-   REPEAT STRIP_TAC THEN
-   IMP_RES_TAC MOD_TIMES THEN
-   PURE_ONCE_REWRITE_TAC [ADD_SYM] THEN
-   IMP_RES_THEN (TRY o SUBS o SPEC (`k:num`)) DIVISION THEN
+   REPEAT STRIP_TAC \\
+   IMP_RES_TAC MOD_TIMES \\
+   PURE_ONCE_REWRITE_TAC [ADD_SYM] \\
+   IMP_RES_THEN (TRY o SUBS o SPEC (`k:num`)) DIVISION \\
    ASM_REWRITE_TAC [SYM(SPEC_ALL ADD_ASSOC)]
    end);
 
@@ -891,157 +886,41 @@ val MOD_LESS = prove(
 
 val MOD_LESS1 = prove(
   `!n. 0 < n ==> a MOD n + 1 <= n`,
-  REPEAT STRIP_TAC THEN IMP_RES_TAC MOD_LESS
-    THEN POP_ASSUM (fn th => ASSUME_TAC (SPEC `a` th))
-    THEN RW_TAC arith_ss []);
+  REPEAT STRIP_TAC \\ IMP_RES_TAC MOD_LESS
+    \\ POP_ASSUM (fn th => ASSUME_TAC (SPEC `a` th))
+    \\ RW_TAC arith_ss []);
 
 val MOD_ZERO = prove(
   `!n. 0 < n /\ 0 < a /\ a <= n /\ (a MOD n = 0) ==> (a = n)`,
-  REPEAT STRIP_TAC THEN Cases_on `a < n`
-    THEN FULL_SIMP_TAC arith_ss [LESS_MOD,GSYM NOT_ZERO_LT_ZERO]);
+  REPEAT STRIP_TAC \\ Cases_on `a < n`
+    \\ FULL_SIMP_TAC arith_ss [LESS_MOD,GSYM NOT_ZERO_LT_ZERO]);
 
 val MOD_PLUS_1 = store_thm("MOD_PLUS_1",
   `!n. 0 < n ==> !x. ((x + 1) MOD n = 0) = (x MOD n + 1 = n)`,
   REPEAT STRIP_TAC
-    THEN Cases_on `n = 1` THEN1 ASM_SIMP_TAC arith_ss [MOD_1]
-    THEN IMP_RES_TAC MOD_PLUS
-    THEN POP_ASSUM (fn th => ONCE_REWRITE_TAC [GSYM th])
-    THEN `1 < n` by ASM_SIMP_TAC arith_ss []
-    THEN ASM_SIMP_TAC bool_ss [LESS_MOD]
-    THEN EQ_TAC THEN STRIP_TAC
-    THENL [
+    \\ Cases_on `n = 1` >> ASM_SIMP_TAC arith_ss [MOD_1]
+    \\ IMP_RES_TAC MOD_PLUS
+    \\ POP_ASSUM (fn th => ONCE_REWRITE_TAC [GSYM th])
+    \\ `1 < n` by ASM_SIMP_TAC arith_ss []
+    \\ ASM_SIMP_TAC bool_ss [LESS_MOD]
+    \\ EQ_TAC \\ STRIP_TAC
+    << [
       `0 < x MOD n + 1` by SIMP_TAC arith_ss []
-        THEN IMP_RES_TAC MOD_LESS1
-        THEN POP_ASSUM (fn th => ASSUME_TAC (SPEC `x` th))
-        THEN IMP_RES_TAC MOD_ZERO,
+        \\ IMP_RES_TAC MOD_LESS1
+        \\ POP_ASSUM (fn th => ASSUME_TAC (SPEC `x` th))
+        \\ IMP_RES_TAC MOD_ZERO,
       ASM_SIMP_TAC bool_ss [ADD_EQ_SUB,SUB_ADD,DIVMOD_ID]]);
 
 val MOD_ADD_1 = store_thm("MOD_ADD_1",
   `!n. 0 < n ==> !x. ~((x + 1) MOD n = 0) ==> ((x + 1) MOD n = x MOD n + 1)`,
   RW_TAC bool_ss [MOD_PLUS_1]
-    THEN IMP_RES_TAC (SPEC `n` DIVISION)
-    THEN PAT_ASSUM `!k. k = k DIV n * n + k MOD n`
-           (fn th => SUBST_OCCS_TAC [([1],SPEC `x` th)])
-    THEN ONCE_REWRITE_TAC [GSYM ADD_ASSOC]
-    THEN POP_ASSUM (fn th => ASSUME_TAC (SPEC `x` th))
-    THEN `x MOD n + 1 < n` by ASM_SIMP_TAC arith_ss []
-    THEN ASM_SIMP_TAC bool_ss [MOD_TIMES,LESS_MOD]);
-
-(* ------------------------------------------------------------------------- *)
-
-val TWO_EXP_GEQ_1 = (numLib.REDUCE_RULE o SPEC `0`) TWOEXP_MONO2;
-
-val LOG2_THM = store_thm("LOG2_THM",
-  `!n. 0 < n ==> ?q. n = 2 ** q + n MOD 2 ** q`,
-  Induct THEN RW_TAC arith_ss []
-    THEN Cases_on `n` THEN FULL_SIMP_TAC arith_ss []
-    THEN1 (EXISTS_TAC `0` THEN SIMP_TAC arith_ss [])
-    THEN EXISTS_TAC `if SUC n' MOD 2 ** q = 2 ** q - 1 then q + 1 else q`
-    THEN RW_TAC std_ss []
-    THENL [
-       POP_ASSUM SUBST_ALL_TAC
-         THEN ASM_SIMP_TAC (arith_ss++numSimps.ARITH_AC_ss)
-                [ZERO_LT_TWOEXP,EXP_ADD,DECIDE ``!n. 0 < n ==> (SUC (n - 1) = n)``],
-       `~(SUC (SUC n') MOD 2 ** q = 0)` by
-          (FULL_SIMP_TAC std_ss [ZERO_LT_TWOEXP,MOD_PLUS_1,ADD1,TWO_EXP_GEQ_1]
-            THEN FULL_SIMP_TAC arith_ss [])
-        THEN ABBREV_TAC `n = SUC n'`
-        THEN FULL_SIMP_TAC arith_ss [ZERO_LT_TWOEXP,MOD_ADD_1,ADD1]]);
-
-val LOG2_exists = prove(
-  `?LOG2. !n. 0 < n ==> (n = 2 ** (LOG2 n) + n MOD 2 ** (LOG2 n))`,
-  EXISTS_TAC `\n. @q. n = 2 ** q + n MOD (2 ** q)`
-    THEN RW_TAC std_ss []
-    THEN SELECT_ELIM_TAC
-    THEN RW_TAC std_ss [LOG2_THM]);
-
-val LOG2 = new_specification ("LOG2", ["LOG2"], LOG2_exists);
-
-val LOG2_2EXPN =
-  (GEN_ALL o
-    SIMP_RULE arith_ss [ZERO_LT_TWOEXP,DECIDE ``!a b. 0 < b ==> 0 < a + b``] o
-   SPEC `2 ** n + r`) LOG2;
-
-val LOG2_2EXPN_0 =
-  (GEN_ALL o SIMP_RULE arith_ss [ZERO_LT_TWOEXP] o SPEC `2 ** n`) LOG2;
-
-val lem = prove(
-  `!a b. a < b ==> (2 ** b MOD 2 ** a = 0)`,
-  REPEAT STRIP_TAC
-    THEN IMP_RES_TAC LESS_ADD
-    THEN POP_ASSUM (SUBST1_TAC o SYM)
-    THEN ASM_SIMP_TAC arith_ss [EXP_ADD,MOD_EQ_0,ZERO_LT_TWOEXP]
-);
-
-val LOG2_POWER = prove(
-  `!q. q = LOG2 (2 ** q)`,
-  STRIP_TAC THEN Cases_on `q < LOG2 (2 ** q)`
-    THENL [
-       POP_ASSUM (fn th => ASSUME_TAC (MATCH_MP TWOEXP_MONO th))
-         THEN ASSUME_TAC (SPEC `q` LOG2_2EXPN_0)
-         THEN FULL_SIMP_TAC arith_ss [],
-       Tactical.REVERSE (Cases_on `LOG2 (2 ** q) < q`) THEN1 DECIDE_TAC
-         THEN IMP_RES_TAC lem
-         THEN PAT_ASSUM `a < b` (fn th => ASSUME_TAC (MATCH_MP TWOEXP_MONO th))
-         THEN ASSUME_TAC (SPEC `q` LOG2_2EXPN_0)
-         THEN FULL_SIMP_TAC arith_ss []]);
-
-val lem2 = DECIDE ``!a b c. a < c /\ b < c ==> a + b < d + (c * 2 + 1)``;
-
-val lem3 = prove(
-  `!a b c d. a < b /\ c < 2 ** (b - 1) ==> 2 ** a + c < 2 ** b + (SUC d)`,
-  Induct_on `b` THEN RW_TAC arith_ss []
-    THEN Cases_on `a = b` THEN FULL_SIMP_TAC arith_ss [ADD1,EXP_ADD]
-    THEN `a < b` by DECIDE_TAC
-    THEN Cases_on `2 ** (b - 1) <= c`
-    THEN FULL_SIMP_TAC arith_ss [ADD1,EXP_ADD]
-    THEN1 (MATCH_MP_TAC lem2 THEN METIS_TAC [TWOEXP_MONO])
-    THEN FULL_SIMP_TAC arith_ss [NOT_LESS_EQUAL]
-    THEN RES_TAC THEN POP_ASSUM (ASSUME_TAC o SPEC `d`)
-    THEN DECIDE_TAC);
-
-val lem4 = prove(
-  `!q n. SUC n < 2 ** q ==> ~(LOG2 (SUC n + 2 ** q) = q - 1)`,
-  REPEAT STRIP_TAC
-    THEN ASSUME_TAC (SPECL [`SUC n`,`q`] LOG2_2EXPN)
-    THEN PAT_ASSUM `LOG2 (SUC n + 2 ** q) = q - 1` SUBST_ALL_TAC
-    THEN Cases_on `q` THEN FULL_SIMP_TAC arith_ss []
-    THEN `(SUC n + 2 ** SUC n') MOD 2 ** n' < 2 ** n'`
-      by ASM_SIMP_TAC arith_ss [MOD_2EXP_LT]
-    THEN FULL_SIMP_TAC arith_ss [ADD1,EXP_ADD]);
-
-val LOG2_UNIQUE = store_thm("LOG2_UNIQUE",
-  `!n q. (?r. (n = 2 ** q + r) /\ r < 2 ** q) ==> (LOG2 n = q)`,
-  RW_TAC arith_ss []
-    THEN Cases_on `q < LOG2 (2 ** q + r)`
-    THENL [
-      IMP_RES_TAC (DECIDE ``!a b. a < b ==> (a + 1 <= b)``)
-        THEN POP_LAST_TAC
-        THEN POP_ASSUM (fn th => ASSUME_TAC (MATCH_MP TWOEXP_MONO2 th))
-        THEN `2 ** q + r < 2 ** (q + 1)` by ASM_SIMP_TAC arith_ss [EXP_ADD]
-        THEN `2 ** q + r < 2 ** LOG2 (2 ** q + r)`
-          by METIS_TAC [lem,LESS_LESS_EQ_TRANS,LESS_TRANS]
-        THEN ASSUME_TAC (SPECL [`r`,`q`] LOG2_2EXPN)
-        THEN FULL_SIMP_TAC (arith_ss++numSimps.ARITH_AC_ss) [],
-      Cases_on `r` THEN1 METIS_TAC [ADD,LOG2_POWER]
-        THEN Cases_on `q = LOG2 (2 ** q + SUC n)`
-        THEN FULL_SIMP_TAC arith_ss []
-        THEN `LOG2 (SUC n + 2 ** q) < q` by DECIDE_TAC
-        THEN `LOG2 (SUC n + 2 ** q) <= q - 1` by DECIDE_TAC
-        THEN IMP_RES_TAC lem4
-        THEN `LOG2 (SUC n + 2 ** q) <= q - 2` by DECIDE_TAC
-        THEN POP_ASSUM (fn th => ASSUME_TAC (MATCH_MP MOD_2EXP_MONO th))
-        THEN `~(q - 1 = 0)` by DECIDE_TAC
-        THEN FULL_SIMP_TAC std_ss
-               [DECIDE ``!n. ~(n - 1 = 0) ==> (SUC (n - 2) = n - 1)``]
-        THEN POP_LAST_TAC
-        THEN POP_ASSUM (ASSUME_TAC o SPEC `SUC n + 2 ** q`)
-        THEN `(SUC n + 2 ** q) MOD 2 ** LOG2 (SUC n + 2 ** q) < 2 ** (q - 1)`
-          by METIS_TAC [MOD_2EXP_LT,LESS_EQ_LESS_TRANS]
-        THEN IMP_RES_TAC lem3 THEN POP_LAST_TAC
-        THEN POP_ASSUM (ASSUME_TAC o SPEC `n`)
-        THEN ASSUME_TAC (SPECL [`SUC n`,`q`] LOG2_2EXPN)
-        THEN FULL_SIMP_TAC arith_ss []]);
+    \\ IMP_RES_TAC (SPEC `n` DIVISION)
+    \\ PAT_ASSUM `!k. k = k DIV n * n + k MOD n`
+         (fn th => SUBST_OCCS_TAC [([1],SPEC `x` th)])
+    \\ ONCE_REWRITE_TAC [GSYM ADD_ASSOC]
+    \\ POP_ASSUM (fn th => ASSUME_TAC (SPEC `x` th))
+    \\ `x MOD n + 1 < n` by ASM_SIMP_TAC arith_ss []
+    \\ ASM_SIMP_TAC bool_ss [MOD_TIMES,LESS_MOD]);
 
 (* ------------------------------------------------------------------------- *)
 
@@ -1049,55 +928,56 @@ val SPEC_EXP1_RULE = (REWRITE_RULE [EXP_1] o SPECL [`x`,`1`]);
 
 val BIT_REVERSE_THM = store_thm("BIT_REVERSE_THM",
   `!x n a. x < n ==> (BIT x (BIT_REVERSE n a) = BIT (n - 1 - x) a)`,
-  Induct_on `n` THEN1 REWRITE_TAC [NOT_LESS_0]
-    THEN RW_TAC std_ss [BIT_REVERSE_def]
-    THEN Cases_on `x = 0`
-    THENL [
-      `2 = 2 ** (SUC 0)` by numLib.REDUCE_TAC THEN POP_ASSUM SUBST1_TAC
-        THEN ASM_SIMP_TAC bool_ss [BIT_def,BITS_SUM2]
-        THEN RW_TAC arith_ss [SBIT_def,BITS_THM],
+  Induct_on `n` >> REWRITE_TAC [NOT_LESS_0]
+    \\ RW_TAC std_ss [BIT_REVERSE_def]
+    \\ Cases_on `x = 0`
+    << [
+      `2 = 2 ** (SUC 0)` by numLib.REDUCE_TAC \\ POP_ASSUM SUBST1_TAC
+        \\ ASM_SIMP_TAC bool_ss [BIT_def,BITS_SUM2]
+        \\ RW_TAC arith_ss [SBIT_def,BITS_THM],
       `!y m n. BIT x (m + n) = BIT (x - 1) (BITS x 1 (m + n))`
           by RW_TAC arith_ss [BIT_def,BITS_COMP_THM2,MIN_DEF]
-        THEN `!b. SBIT b 0 < 2` by RW_TAC arith_ss [SBIT_def]
-        THEN `!y b. BIT x (y * 2 + SBIT b 0) = BIT (x - 1) y`
-          by (ASM_SIMP_TAC arith_ss [SPEC_EXP1_RULE BITS_SUM,
-                                     SPEC_EXP1_RULE BITS_ZERO4]
-                THEN SIMP_TAC arith_ss [BIT_def,BITS_COMP_THM2])
-        THEN `x - 1 < n` by DECIDE_TAC
-        THEN ASM_SIMP_TAC std_ss []
-        THEN Cases_on `n = 0` THEN1 ASM_SIMP_TAC arith_ss []
-        THEN `1 <= n /\ 1 <= x` by DECIDE_TAC
-        THEN ASM_SIMP_TAC std_ss [ADD1,SUB_SUB,ADD_SUB,SUB_ADD]]);
+        \\ `!b. SBIT b 0 < 2` by RW_TAC arith_ss [SBIT_def]
+        \\ `!y b. BIT x (y * 2 + SBIT b 0) = BIT (x - 1) y`
+        by (ASM_SIMP_TAC arith_ss
+                  [SPEC_EXP1_RULE BITS_SUM, SPEC_EXP1_RULE BITS_ZERO4]
+             \\ SIMP_TAC arith_ss [BIT_def,BITS_COMP_THM2])
+        \\ `x - 1 < n` by DECIDE_TAC
+        \\ ASM_SIMP_TAC std_ss []
+        \\ Cases_on `n = 0` >> ASM_SIMP_TAC arith_ss []
+        \\ `1 <= n /\ 1 <= x` by DECIDE_TAC
+        \\ ASM_SIMP_TAC std_ss [ADD1,SUB_SUB,ADD_SUB,SUB_ADD]]);
 
 (* ------------------------------------------------------------------------- *)
 
 val BIT_MODIFY_LT_2EXP = prove(
   `!n f a. BIT_MODIFY n f a < 2 ** n`,
   Induct_on `n`
-    THEN RW_TAC bool_ss [ADD_0,TIMES2,LESS_IMP_LESS_ADD,LESS_MONO_ADD,
-           BIT_MODIFY_def,SBIT_def,EXP] THEN REDUCE_TAC);
+    \\ RW_TAC bool_ss [ADD_0,TIMES2,LESS_IMP_LESS_ADD,LESS_MONO_ADD,
+           BIT_MODIFY_def,SBIT_def,EXP] \\ REDUCE_TAC);
 
 val BIT_MODIFY_LEM = prove(
   `!n f a. BIT n (BIT_MODIFY (SUC n) f a) = f n (BIT n a)`,
   RW_TAC arith_ss [SBIT_def,BIT_MODIFY_def,NOT_BIT]
-    THEN1 SIMP_TAC arith_ss [BIT_def,BITS_THM,SUC_SUB,
-            REWRITE_RULE [BIT_MODIFY_LT_2EXP]
-              (SPECL [`BIT_MODIFY n f a`,`2 ** n`] DIV_MULT_1)]
-    THEN SIMP_TAC arith_ss [BITS_THM,LESS_DIV_EQ_ZERO,BIT_MODIFY_LT_2EXP,SUC_SUB]);
+    >> SIMP_TAC arith_ss [BIT_def,BITS_THM,SUC_SUB,
+         REWRITE_RULE [BIT_MODIFY_LT_2EXP]
+           (SPECL [`BIT_MODIFY n f a`,`2 ** n`] DIV_MULT_1)]
+    \\ SIMP_TAC arith_ss [BITS_THM,LESS_DIV_EQ_ZERO,BIT_MODIFY_LT_2EXP,SUC_SUB]
+);
 
 val BIT_MODIFY_THM = store_thm("BIT_MODIFY_THM",
   `!x n f a. x < n ==> (BIT x (BIT_MODIFY n f a) = f x (BIT x a))`,
-  Induct_on `n` THEN REPEAT STRIP_TAC THEN1 FULL_SIMP_TAC arith_ss []
-    THEN Cases_on `x = n` THEN1 ASM_REWRITE_TAC [BIT_MODIFY_LEM]
-    THEN `x < n` by ASM_SIMP_TAC arith_ss []
-    THEN RW_TAC arith_ss [BIT_MODIFY_def,SBIT_def]
-    THEN LEFT_REWRITE_TAC [BIT_def] THEN ASM_REWRITE_TAC [BITS_THM]
-    THEN IMP_RES_TAC LESS_EXP_MULT2 THEN POP_LAST_TAC
-    THEN ASM_SIMP_TAC bool_ss [ZERO_LT_TWOEXP,ADD_DIV_ADD_DIV,
-           TWO_SUC_SUB,GSYM ADD1,EXP,ONCE_REWRITE_RULE [MULT_COMM]
-           (REWRITE_RULE [DECIDE (Term `0 < 2`)] (SPEC `2` MOD_TIMES))]
-    THEN SUBST_OCCS_TAC [([2],SYM (SPEC `x` TWO_SUC_SUB))]
-    THEN ASM_SIMP_TAC bool_ss [GSYM BITS_THM,GSYM BIT_def]);
+  Induct_on `n` \\ REPEAT STRIP_TAC >> FULL_SIMP_TAC arith_ss []
+    \\ Cases_on `x = n` >> ASM_REWRITE_TAC [BIT_MODIFY_LEM]
+    \\ `x < n` by ASM_SIMP_TAC arith_ss []
+    \\ RW_TAC arith_ss [BIT_MODIFY_def,SBIT_def]
+    \\ LEFT_REWRITE_TAC [BIT_def] \\ ASM_REWRITE_TAC [BITS_THM]
+    \\ IMP_RES_TAC LESS_EXP_MULT2 \\ POP_LAST_TAC
+    \\ ASM_SIMP_TAC bool_ss [ZERO_LT_TWOEXP,ADD_DIV_ADD_DIV,
+         TWO_SUC_SUB,GSYM ADD1,EXP,ONCE_REWRITE_RULE [MULT_COMM]
+         (REWRITE_RULE [DECIDE (Term `0 < 2`)] (SPEC `2` MOD_TIMES))]
+    \\ SUBST_OCCS_TAC [([2],SYM (SPEC `x` TWO_SUC_SUB))]
+    \\ ASM_SIMP_TAC bool_ss [GSYM BITS_THM,GSYM BIT_def]);
 
 (* ------------------------------------------------------------------------- *)
 
